SymbolicLean/Examples.lean
@@ -1,0 +1,4 @@
+import SymbolicLean.Examples.Matrices
+import SymbolicLean.Examples.Negative
+import SymbolicLean.Examples.Scalars
+import SymbolicLean.Examples.Solvers
