SymbolicLean/Examples/Negative.lean
@@ -1,0 +1,42 @@
+import SymbolicLean
+
+open SymbolicLean
+
+/--
+error: failed to synthesize instance of type class
+  HMul (Term (SymSort.matrix (DomainDesc.ground GroundDom.QQ) (Dim.static 2) (Dim.static 2)))
+    (Term (SymSort.matrix (DomainDesc.ground GroundDom.QQ) (Dim.static 3) (Dim.static 1))) ?m.30
+
+Hint: Type class instance resolution failures can be inspected with the `set_option trace.Meta.synthInstance true` command.
+-/
+#guard_msgs in
+example : Term (.matrix (.ground .QQ) (.static 2) (.static 1)) :=
+  let A : SymDecl (.matrix (.ground .QQ) (.static 2) (.static 2)) := { name := `A }
+  let v : SymDecl (.matrix (.ground .QQ) (.static 3) (.static 1)) := { name := `v }
+  term![A * v]
+
+/--
+error: failed to synthesize instance of type class
+  InterpretsField (DomainDesc.ground GroundDom.ZZ)
+
+Hint: Type class instance resolution failures can be inspected with the `set_option trace.Meta.synthInstance true` command.
+-/
+#guard_msgs in
+example {s : SessionTok} (matrix : SymExpr s (.matrix (.ground .ZZ) (.static 2) (.static 2))) :
+    SymPyM s (SymExpr s (.matrix (.ground .ZZ) (.static 2) (.static 2))) :=
+  inv matrix
+
+/--
+error: Application type mismatch: The last
+  x
+argument has type
+  Term (SymSort.scalar (DomainDesc.ground GroundDom.ZZ))
+but is expected to have type
+  SymDecl (SymSort.scalar ?m.7)
+in the application
+  @diff (SymSort.scalar (DomainDesc.ground GroundDom.ZZ)) ?m.7 x x
+-/
+#guard_msgs in
+example : Term (.scalar (.ground .ZZ)) :=
+  let x : Term (.scalar (.ground .ZZ)) := (1 : Term (.scalar (.ground .ZZ)))
+  diff x x
